src/tools/parallelcomposition/instantiations/end_to_end_correctnessScript.sml
@@ -35,7 +35,7 @@ val end_to_end_correctness_thm = store_thm(
   !mu ms mla (birprog:'observation_type bir_program_t) (arm8prog:((64 word)# (8 word) list) list) n' lo c_st c_addr_labels
       (AMTrn:('attevent + 'ceventS, 'cstate) mctrel) Re0 NRe0 i Re NRe (Sym:(Var_t -> bool))
       (Sym':(Var_t -> bool)) (P:(bir_exp_t + DYpred -> bool)) (P':(bir_exp_t + DYpred -> bool))
-      (T0:(sbir_event, real,(bir_var_t, bir_exp_t) symb_interpret_t) stree) (Tre:(sbir_event, real,(bir_var_t, bir_exp_t) symb_interpret_t) stree) (sbir_Ded:(bir_exp_t) tded) (sapic_Ded:(SapicTerm_t) tded) .
+      (T0:(sbir_event, real,(bir_var_t, bir_exp_t) symb_interpret_t) stree) (Tre:(sbir_event, real,(bir_var_t, bir_exp_t) symb_interpret_t) stree) (sbir_Ded:(bir_exp_t) tded)  .
 
     bir_is_lifted_prog arm8_bmr mu arm8prog birprog ==>
     bmr_rel arm8_bmr ((InterpretStOne:(sbir_event, real,(bir_var_t, bir_exp_t) symb_interpret_t) stree -> bir_state_t) T0) ms ==>
@@ -61,17 +61,17 @@ val end_to_end_correctness_thm = store_thm(
         (comptraces_tree (symbolic_tree_multi_transitions_with_symb,sbir_Ded) (DYmultranrel,DYdeduction) composeDedOverApprox (Sym,P,T0,ESt) (Sym',P',Tre,ESt))
        ) ∧
        (TransDisable composeDedOverApprox (symbolic_tree_multi_transitions_with_symb,sbir_Ded) (DYmultranrel,DYdeduction)) ∧
-       (TransEnable composeDedOverApproxSapic (sapic_position_multi_transitions_with_symb,sapic_Ded) (DYmultranrel,DYdeduction))
+       (TransEnable composeDedOverApproxSapic (sapic_position_multi_transitions_with_symb,SPdeduction) (DYmultranrel,DYdeduction))
        ) ==>
        (
        ((IMAGE (MAP sbirEvent_vs_DY_to_sapicFact_vs_DY) (comptraces_tree (symbolic_tree_multi_transitions_with_symb,sbir_Ded) (DYmultranrel,DYdeduction) composeDedOverApprox (Sym,P,T0,ESt) (Sym',P',Tre,ESt))) ⊆
-        (comptraces_sapic (sapic_position_multi_transitions_with_symb,sapic_Ded) (DYmultranrel,DYdeduction) composeDedOverApproxSapic (Sym,(IMAGE (SUM_MAP translate_birexp_to_sapicterm I) P),(Pconfig ((symbtree_to_sapic T0),0,Re0,NRe0)),ESt) (Sym',(IMAGE (SUM_MAP translate_birexp_to_sapicterm I) P'),(Pconfig ((symbtree_to_sapic Tre),i,Re,NRe)),ESt))
+        (comptraces_sapic (sapic_position_multi_transitions_with_symb,SPdeduction) (DYmultranrel,DYdeduction) composeDedOverApproxSapic (Sym,(IMAGE (SUM_MAP translate_BinPred_to_SPpred I) P),(Pconfig ((symbtree_to_sapic T0),0,Re0,NRe0)),ESt) (Sym',(IMAGE (SUM_MAP translate_BinPred_to_SPpred I) P'),(Pconfig ((symbtree_to_sapic Tre),i,Re,NRe)),ESt))
        ) ∧
-       (TransDisable composeDedOverApproxSapic (sapic_position_multi_transitions_with_symb,sapic_Ded) (DYmultranrel,DYdeduction)) ∧
-       (TransEnable composeDedOverApproxSapic (sapic_position_multi_transitions_with_symb,sapic_Ded) (DYmultranrel,DYdeduction))
+       (TransDisable composeDedOverApproxSapic (sapic_position_multi_transitions_with_symb,SPdeduction) (DYmultranrel,DYdeduction)) ∧
+       (TransEnable composeDedOverApproxSapic (sapic_position_multi_transitions_with_symb,SPdeduction) (DYmultranrel,DYdeduction))
        ) ==>
-       (comptraces (sapic_position_multi_transitions_with_symb,sapic_Ded) (DYmultranrel,DYdeduction) composeDedOverApproxSapic (Sym,(IMAGE (SUM_MAP translate_birexp_to_sapicterm I) P),(Pconfig ((symbtree_to_sapic T0),0,Re0,NRe0)),ESt) (Sym',(IMAGE (SUM_MAP translate_birexp_to_sapicterm I) P'),(Pconfig ((symbtree_to_sapic Tre),i,Re,NRe)),ESt)) =
-       (sapic_plus_traces sapic_plus_position_multi_transitions_with_symb (Sym,(IMAGE (SUM_MAP translate_birexp_to_sapicterm I) P),(Pconfig_plus ((symbtree_to_sapic T0),0,Re0,NRe0))) (Sym',(IMAGE (SUM_MAP translate_birexp_to_sapicterm I) P'),(Pconfig_plus ((symbtree_to_sapic Tre),i,Re,NRe))))
+       (comptraces (sapic_position_multi_transitions_with_symb,SPdeduction) (DYmultranrel,DYdeduction) composeDedOverApproxSapic (Sym,(IMAGE (SUM_MAP translate_BinPred_to_SPpred I) P),(Pconfig ((symbtree_to_sapic T0),0,Re0,NRe0)),ESt) (Sym',(IMAGE (SUM_MAP translate_BinPred_to_SPpred I) P'),(Pconfig ((symbtree_to_sapic Tre),i,Re,NRe)),ESt)) =
+       (sapic_plus_traces sapic_plus_position_multi_transitions_with_symb (Sym,(IMAGE (SUM_MAP translate_BinPred_to_SPpred I) P),(Pconfig_plus ((symbtree_to_sapic T0),0,Re0,NRe0))) (Sym',(IMAGE (SUM_MAP translate_BinPred_to_SPpred I) P'),(Pconfig_plus ((symbtree_to_sapic Tre),i,Re,NRe))))
     )
 
     ``,
@@ -121,7 +121,7 @@ val end_to_end_correctness_Winit_thm = store_thm(
   !mu ms mla n' lo c_st c_addr_labels
       (AMTrn:('attevent + 'ceventS, 'cstate) mctrel) Re0 NRe0 i Re NRe (Sym:(Var_t -> bool))
       (Sym':(Var_t -> bool)) (P:(bir_exp_t + DYpred -> bool)) (P':(bir_exp_t + DYpred -> bool))
-      (T0:(sbir_event, real,(bir_var_t, bir_exp_t) symb_interpret_t) stree) (Tre:(sbir_event, real,(bir_var_t, bir_exp_t) symb_interpret_t) stree) (sbir_Ded:(bir_exp_t) tded) (sapic_Ded:(SapicTerm_t) tded) .
+      (T0:(sbir_event, real,(bir_var_t, bir_exp_t) symb_interpret_t) stree) (Tre:(sbir_event, real,(bir_var_t, bir_exp_t) symb_interpret_t) stree) (sbir_Ded:(bir_exp_t) tded)  .
 
     ^lifter_Winit_t ==>
     bmr_rel arch_Winit ((InterpretStOne:(sbir_event, real,(bir_var_t, bir_exp_t) symb_interpret_t) stree -> bir_state_t) T0) ms ==>
@@ -147,17 +147,17 @@ val end_to_end_correctness_Winit_thm = store_thm(
         (comptraces_tree (symbolic_tree_multi_transitions_with_symb,sbir_Ded) (DYmultranrel,DYdeduction) composeDedOverApprox (Sym,P,T0,ESt) (Sym',P',Tre,ESt))
        ) ∧
        (TransDisable composeDedOverApprox (symbolic_tree_multi_transitions_with_symb,sbir_Ded) (DYmultranrel,DYdeduction)) ∧
-       (TransEnable composeDedOverApproxSapic (sapic_position_multi_transitions_with_symb,sapic_Ded) (DYmultranrel,DYdeduction))
+       (TransEnable composeDedOverApproxSapic (sapic_position_multi_transitions_with_symb,SPdeduction) (DYmultranrel,DYdeduction))
        ) ==>
        (
        ((IMAGE (MAP sbirEvent_vs_DY_to_sapicFact_vs_DY) (comptraces_tree (symbolic_tree_multi_transitions_with_symb,sbir_Ded) (DYmultranrel,DYdeduction) composeDedOverApprox (Sym,P,T0,ESt) (Sym',P',Tre,ESt))) ⊆
-        (comptraces_sapic (sapic_position_multi_transitions_with_symb,sapic_Ded) (DYmultranrel,DYdeduction) composeDedOverApproxSapic (Sym,(IMAGE (SUM_MAP translate_birexp_to_sapicterm I) P),(Pconfig ((symbtree_to_sapic T0),0,Re0,NRe0)),ESt) (Sym',(IMAGE (SUM_MAP translate_birexp_to_sapicterm I) P'),(Pconfig ((symbtree_to_sapic Tre),i,Re,NRe)),ESt))
+        (comptraces_sapic (sapic_position_multi_transitions_with_symb,SPdeduction) (DYmultranrel,DYdeduction) composeDedOverApproxSapic (Sym,(IMAGE (SUM_MAP translate_BinPred_to_SPpred I) P),(Pconfig ((symbtree_to_sapic T0),0,Re0,NRe0)),ESt) (Sym',(IMAGE (SUM_MAP translate_BinPred_to_SPpred I) P'),(Pconfig ((symbtree_to_sapic Tre),i,Re,NRe)),ESt))
        ) ∧
-       (TransDisable composeDedOverApproxSapic (sapic_position_multi_transitions_with_symb,sapic_Ded) (DYmultranrel,DYdeduction)) ∧
-       (TransEnable composeDedOverApproxSapic (sapic_position_multi_transitions_with_symb,sapic_Ded) (DYmultranrel,DYdeduction))
+       (TransDisable composeDedOverApproxSapic (sapic_position_multi_transitions_with_symb,SPdeduction) (DYmultranrel,DYdeduction)) ∧
+       (TransEnable composeDedOverApproxSapic (sapic_position_multi_transitions_with_symb,SPdeduction) (DYmultranrel,DYdeduction))
        ) ==>
-       (comptraces (sapic_position_multi_transitions_with_symb,sapic_Ded) (DYmultranrel,DYdeduction) composeDedOverApproxSapic (Sym,(IMAGE (SUM_MAP translate_birexp_to_sapicterm I) P),(Pconfig ((symbtree_to_sapic T0),0,Re0,NRe0)),ESt) (Sym',(IMAGE (SUM_MAP translate_birexp_to_sapicterm I) P'),(Pconfig ((symbtree_to_sapic Tre),i,Re,NRe)),ESt)) =
-       (sapic_plus_traces sapic_plus_position_multi_transitions_with_symb (Sym,(IMAGE (SUM_MAP translate_birexp_to_sapicterm I) P),(Pconfig_plus ((symbtree_to_sapic T0),0,Re0,NRe0))) (Sym',(IMAGE (SUM_MAP translate_birexp_to_sapicterm I) P'),(Pconfig_plus ((symbtree_to_sapic Tre),i,Re,NRe))))
+       (comptraces (sapic_position_multi_transitions_with_symb,SPdeduction) (DYmultranrel,DYdeduction) composeDedOverApproxSapic (Sym,(IMAGE (SUM_MAP translate_BinPred_to_SPpred I) P),(Pconfig ((symbtree_to_sapic T0),0,Re0,NRe0)),ESt) (Sym',(IMAGE (SUM_MAP translate_BinPred_to_SPpred I) P'),(Pconfig ((symbtree_to_sapic Tre),i,Re,NRe)),ESt)) =
+       (sapic_plus_traces sapic_plus_position_multi_transitions_with_symb (Sym,(IMAGE (SUM_MAP translate_BinPred_to_SPpred I) P),(Pconfig_plus ((symbtree_to_sapic T0),0,Re0,NRe0))) (Sym',(IMAGE (SUM_MAP translate_BinPred_to_SPpred I) P'),(Pconfig_plus ((symbtree_to_sapic Tre),i,Re,NRe))))
     )
 
 
@@ -202,7 +202,7 @@ val end_to_end_correctness_Wresp_thm = store_thm(
   !mu ms mla n' lo c_st c_addr_labels
       (AMTrn:('attevent + 'ceventS, 'cstate) mctrel) Re0 NRe0 i Re NRe (Sym:(Var_t -> bool))
       (Sym':(Var_t -> bool)) (P:(bir_exp_t + DYpred -> bool)) (P':(bir_exp_t + DYpred -> bool))
-      (T0:(sbir_event, real,(bir_var_t, bir_exp_t) symb_interpret_t) stree) (Tre:(sbir_event, real,(bir_var_t, bir_exp_t) symb_interpret_t) stree) (sbir_Ded:(bir_exp_t) tded) (sapic_Ded:(SapicTerm_t) tded) .
+      (T0:(sbir_event, real,(bir_var_t, bir_exp_t) symb_interpret_t) stree) (Tre:(sbir_event, real,(bir_var_t, bir_exp_t) symb_interpret_t) stree) (sbir_Ded:(bir_exp_t) tded)  .
 
     ^lifter_Wresp_t ==>
     bmr_rel arch_Wresp ((InterpretStOne:(sbir_event, real,(bir_var_t, bir_exp_t) symb_interpret_t) stree -> bir_state_t) T0) ms ==>
@@ -228,17 +228,17 @@ val end_to_end_correctness_Wresp_thm = store_thm(
         (comptraces_tree (symbolic_tree_multi_transitions_with_symb,sbir_Ded) (DYmultranrel,DYdeduction) composeDedOverApprox (Sym,P,T0,ESt) (Sym',P',Tre,ESt))
        ) ∧
        (TransDisable composeDedOverApprox (symbolic_tree_multi_transitions_with_symb,sbir_Ded) (DYmultranrel,DYdeduction)) ∧
-       (TransEnable composeDedOverApproxSapic (sapic_position_multi_transitions_with_symb,sapic_Ded) (DYmultranrel,DYdeduction))
+       (TransEnable composeDedOverApproxSapic (sapic_position_multi_transitions_with_symb,SPdeduction) (DYmultranrel,DYdeduction))
        ) ==>
        (
        ((IMAGE (MAP sbirEvent_vs_DY_to_sapicFact_vs_DY) (comptraces_tree (symbolic_tree_multi_transitions_with_symb,sbir_Ded) (DYmultranrel,DYdeduction) composeDedOverApprox (Sym,P,T0,ESt) (Sym',P',Tre,ESt))) ⊆
-        (comptraces_sapic (sapic_position_multi_transitions_with_symb,sapic_Ded) (DYmultranrel,DYdeduction) composeDedOverApproxSapic (Sym,(IMAGE (SUM_MAP translate_birexp_to_sapicterm I) P),(Pconfig ((symbtree_to_sapic T0),0,Re0,NRe0)),ESt) (Sym',(IMAGE (SUM_MAP translate_birexp_to_sapicterm I) P'),(Pconfig ((symbtree_to_sapic Tre),i,Re,NRe)),ESt))
+        (comptraces_sapic (sapic_position_multi_transitions_with_symb,SPdeduction) (DYmultranrel,DYdeduction) composeDedOverApproxSapic (Sym,(IMAGE (SUM_MAP translate_BinPred_to_SPpred I) P),(Pconfig ((symbtree_to_sapic T0),0,Re0,NRe0)),ESt) (Sym',(IMAGE (SUM_MAP translate_BinPred_to_SPpred I) P'),(Pconfig ((symbtree_to_sapic Tre),i,Re,NRe)),ESt))
        ) ∧
-       (TransDisable composeDedOverApproxSapic (sapic_position_multi_transitions_with_symb,sapic_Ded) (DYmultranrel,DYdeduction)) ∧
-       (TransEnable composeDedOverApproxSapic (sapic_position_multi_transitions_with_symb,sapic_Ded) (DYmultranrel,DYdeduction))
+       (TransDisable composeDedOverApproxSapic (sapic_position_multi_transitions_with_symb,SPdeduction) (DYmultranrel,DYdeduction)) ∧
+       (TransEnable composeDedOverApproxSapic (sapic_position_multi_transitions_with_symb,SPdeduction) (DYmultranrel,DYdeduction))
        ) ==>
-       (comptraces (sapic_position_multi_transitions_with_symb,sapic_Ded) (DYmultranrel,DYdeduction) composeDedOverApproxSapic (Sym,(IMAGE (SUM_MAP translate_birexp_to_sapicterm I) P),(Pconfig ((symbtree_to_sapic T0),0,Re0,NRe0)),ESt) (Sym',(IMAGE (SUM_MAP translate_birexp_to_sapicterm I) P'),(Pconfig ((symbtree_to_sapic Tre),i,Re,NRe)),ESt)) =
-       (sapic_plus_traces sapic_plus_position_multi_transitions_with_symb (Sym,(IMAGE (SUM_MAP translate_birexp_to_sapicterm I) P),(Pconfig_plus ((symbtree_to_sapic T0),0,Re0,NRe0))) (Sym',(IMAGE (SUM_MAP translate_birexp_to_sapicterm I) P'),(Pconfig_plus ((symbtree_to_sapic Tre),i,Re,NRe))))
+       (comptraces (sapic_position_multi_transitions_with_symb,SPdeduction) (DYmultranrel,DYdeduction) composeDedOverApproxSapic (Sym,(IMAGE (SUM_MAP translate_BinPred_to_SPpred I) P),(Pconfig ((symbtree_to_sapic T0),0,Re0,NRe0)),ESt) (Sym',(IMAGE (SUM_MAP translate_BinPred_to_SPpred I) P'),(Pconfig ((symbtree_to_sapic Tre),i,Re,NRe)),ESt)) =
+       (sapic_plus_traces sapic_plus_position_multi_transitions_with_symb (Sym,(IMAGE (SUM_MAP translate_BinPred_to_SPpred I) P),(Pconfig_plus ((symbtree_to_sapic T0),0,Re0,NRe0))) (Sym',(IMAGE (SUM_MAP translate_BinPred_to_SPpred I) P'),(Pconfig_plus ((symbtree_to_sapic Tre),i,Re,NRe))))
     )
 
 
@@ -278,7 +278,7 @@ val two_sbirs_DY_comptraces_def = Define `
                                `;
 
 val two_sapics_DY_comptraces_thm =
-INST_TYPE [``:'symb`` |-> ``:Var_t``,``:'pred1`` |-> ``:(SapicTerm_t + DYpred)``,``:'state1`` |-> ``:(sapic_position_configuration_t # DYstate)``,``:'event1`` |-> ``:(SapicFact_t + (Name_t, Sig_t, Var_t) sync_event)``,``:'pred2`` |-> ``:(SapicTerm_t + DYpred)``,``:'state2`` |-> ``:(sapic_position_configuration_t # DYstate)``,``:'event2`` |-> ``:(SapicFact_t + (Name_t, Sig_t, Var_t) sync_event)``,``:'eventS`` |-> ``:(DYnsyc_event + (Name_t, Sig_t, Var_t) sync_event)``] derived_rules_generaldeductionTheory.comptraces_def;
+INST_TYPE [``:'symb`` |-> ``:Var_t``,``:'pred1`` |-> ``:(SPpred + DYpred)``,``:'state1`` |-> ``:(sapic_position_configuration_t # DYstate)``,``:'event1`` |-> ``:(SapicFact_t + (Name_t, Sig_t, Var_t) sync_event)``,``:'pred2`` |-> ``:(SPpred + DYpred)``,``:'state2`` |-> ``:(sapic_position_configuration_t # DYstate)``,``:'event2`` |-> ``:(SapicFact_t + (Name_t, Sig_t, Var_t) sync_event)``,``:'eventS`` |-> ``:(DYnsyc_event + (Name_t, Sig_t, Var_t) sync_event)``] derived_rules_generaldeductionTheory.comptraces_def;
 val two_sapics_DY_comptraces_t = (fst o strip_comb o fst o dest_eq o snd o strip_forall o concl) two_sapics_DY_comptraces_thm;
 val two_sapics_DY_comptraces_def = Define `
     two_sapics_DY_comptraces = ^(two_sapics_DY_comptraces_t)
@@ -304,7 +304,7 @@ val end_to_end_correctness_Winit_vs_Wresp_vs_attacker_thm = store_thm(
        (rAMTrn:(('attevent + 'ceventS), 'cstate) mctrel)
        iRe0 iNRe0 ii iRe iNRe (iT0:(sbir_event, real,(bir_var_t, bir_exp_t) symb_interpret_t) stree) (iTre:(sbir_event, real,(bir_var_t, bir_exp_t) symb_interpret_t) stree)
        rRe0 rNRe0 ri rRe rNRe (rT0:(sbir_event, real,(bir_var_t, bir_exp_t) symb_interpret_t) stree) (rTre:(sbir_event, real,(bir_var_t, bir_exp_t) symb_interpret_t) stree)
-        (wded3Tr:(bir_exp_t + DYpred) tded) (wded4Tr:((bir_exp_t + DYpred)+(bir_exp_t + DYpred)) tded) (wded3Sp:(SapicTerm_t + DYpred) tded) (wded4Sp:((SapicTerm_t + DYpred)+(SapicTerm_t + DYpred)) tded) (sbir_Ded:(bir_exp_t) tded) (sapic_Ded:(SapicTerm_t) tded) 
+        (wded3Tr:(bir_exp_t + DYpred) tded) (wded4Tr:((bir_exp_t + DYpred)+(bir_exp_t + DYpred)) tded) (wded3Sp:(SPpred + DYpred) tded) (wded4Sp:((SPpred + DYpred)+(SPpred + DYpred)) tded) (sbir_Ded:(bir_exp_t) tded)  
        (Sym:(Var_t -> bool)) (Sym':(Var_t -> bool)) (P:((bir_exp_t + DYpred) -> bool)) (P':((bir_exp_t + DYpred) -> bool)).
 
     ^lifter_Winit_t ==>  
@@ -348,7 +348,7 @@ val end_to_end_correctness_Winit_vs_Wresp_vs_attacker_thm = store_thm(
          (Sym,((IMAGE INL P):((bir_exp_t + DYpred) + (bir_exp_t + DYpred) -> bool)),(iT0,ESt),(rT0,ESt)) (Sym',((IMAGE INL P'):((bir_exp_t + DYpred) + (bir_exp_t + DYpred) -> bool)),(iTre,ESt),(rTre,ESt)))
        )∧
        (TransDisable composeDedOverApprox (symbolic_tree_multi_transitions_with_symb,sbir_Ded) (DYmultranrel,DYdeduction)) ∧
-       (TransEnable composeDedOverApproxSapic (sapic_position_multi_transitions_with_symb,sapic_Ded) (DYmultranrel,DYdeduction))
+       (TransEnable composeDedOverApproxSapic (sapic_position_multi_transitions_with_symb,SPdeduction) (DYmultranrel,DYdeduction))
 ) ==>
   (
        ((IMAGE (MAP (OPTION_MAP (SUM_MAP sbirEvent_vs_DY_to_sapicFact_vs_DY_no_option sbirEvent_vs_DY_to_sapicFact_vs_DY_no_option)))
@@ -356,26 +356,26 @@ val end_to_end_correctness_Winit_vs_Wresp_vs_attacker_thm = store_thm(
           ((symbolicParlComp (symbolic_tree_multi_transitions_with_symb,sbir_Ded) (DYmultranrel,DYdeduction) composeDedOverApprox),wded3Tr) wded4Tr
           (Sym,((IMAGE INL P):((bir_exp_t + DYpred) + (bir_exp_t + DYpred) -> bool)),(iT0,ESt),(rT0,ESt)) (Sym',((IMAGE INL P'):((bir_exp_t + DYpred) + (bir_exp_t + DYpred) -> bool)),(iTre,ESt),(rTre,ESt))))
         ⊆
-        (two_sapics_DY_comptraces ((symbolicParlComp (sapic_position_multi_transitions_with_symb,sapic_Ded) (DYmultranrel,DYdeduction) composeDedOverApproxSapic),wded3Sp)
-         ((symbolicParlComp (sapic_position_multi_transitions_with_symb,sapic_Ded) (DYmultranrel,DYdeduction) composeDedOverApproxSapic),wded3Sp) wded4Sp
-         (Sym,((IMAGE INL (IMAGE (SUM_MAP translate_birexp_to_sapicterm I) P)):((SapicTerm_t + DYpred) + (SapicTerm_t + DYpred) -> bool)),((Pconfig ((symbtree_to_sapic iT0),0,iRe0,iNRe0)),ESt),((Pconfig ((symbtree_to_sapic rT0),0,rRe0,rNRe0)),ESt))
-         (Sym',((IMAGE INL (IMAGE (SUM_MAP translate_birexp_to_sapicterm I) P')):((SapicTerm_t + DYpred) + (SapicTerm_t + DYpred) -> bool)),((Pconfig ((symbtree_to_sapic iTre),ii,iRe,iNRe)),ESt),((Pconfig ((symbtree_to_sapic rTre),ri,rRe,rNRe)),ESt)))
+        (two_sapics_DY_comptraces ((symbolicParlComp (sapic_position_multi_transitions_with_symb,SPdeduction) (DYmultranrel,DYdeduction) composeDedOverApproxSapic),wded3Sp)
+         ((symbolicParlComp (sapic_position_multi_transitions_with_symb,SPdeduction) (DYmultranrel,DYdeduction) composeDedOverApproxSapic),wded3Sp) wded4Sp
+         (Sym,((IMAGE INL (IMAGE (SUM_MAP translate_BinPred_to_SPpred I) P)):((SPpred + DYpred) + (SPpred + DYpred) -> bool)),((Pconfig ((symbtree_to_sapic iT0),0,iRe0,iNRe0)),ESt),((Pconfig ((symbtree_to_sapic rT0),0,rRe0,rNRe0)),ESt))
+         (Sym',((IMAGE INL (IMAGE (SUM_MAP translate_BinPred_to_SPpred I) P')):((SPpred + DYpred) + (SPpred + DYpred) -> bool)),((Pconfig ((symbtree_to_sapic iTre),ii,iRe,iNRe)),ESt),((Pconfig ((symbtree_to_sapic rTre),ri,rRe,rNRe)),ESt)))
        )∧
-       (TransDisable composeDedOverApproxSapic (sapic_position_multi_transitions_with_symb,sapic_Ded) (DYmultranrel,DYdeduction)) ∧
-       (TransEnable composeDedOverApproxSapic (sapic_position_multi_transitions_with_symb,sapic_Ded) (DYmultranrel,DYdeduction))
+       (TransDisable composeDedOverApproxSapic (sapic_position_multi_transitions_with_symb,SPdeduction) (DYmultranrel,DYdeduction)) ∧
+       (TransEnable composeDedOverApproxSapic (sapic_position_multi_transitions_with_symb,SPdeduction) (DYmultranrel,DYdeduction))
        ) ==>
        (
-       (two_sapics_DY_comptraces ((symbolicParlComp (sapic_position_multi_transitions_with_symb,sapic_Ded) (DYmultranrel,DYdeduction) composeDedOverApproxSapic),wded3Sp)
-        ((symbolicParlComp (sapic_position_multi_transitions_with_symb,sapic_Ded) (DYmultranrel,DYdeduction) composeDedOverApproxSapic),wded3Sp) wded4Sp
-        (Sym,((IMAGE INL (IMAGE (SUM_MAP translate_birexp_to_sapicterm I) P)):((SapicTerm_t + DYpred) + (SapicTerm_t + DYpred) -> bool)),((Pconfig ((symbtree_to_sapic iT0),0,iRe0,iNRe0)),ESt),((Pconfig ((symbtree_to_sapic rT0),0,rRe0,rNRe0)),ESt))
-        (Sym',((IMAGE INL (IMAGE (SUM_MAP translate_birexp_to_sapicterm I) P')):((SapicTerm_t + DYpred) + (SapicTerm_t + DYpred) -> bool)),((Pconfig ((symbtree_to_sapic iTre),ii,iRe,iNRe)),ESt),((Pconfig ((symbtree_to_sapic rTre),ri,rRe,rNRe)),ESt)))
+       (two_sapics_DY_comptraces ((symbolicParlComp (sapic_position_multi_transitions_with_symb,SPdeduction) (DYmultranrel,DYdeduction) composeDedOverApproxSapic),wded3Sp)
+        ((symbolicParlComp (sapic_position_multi_transitions_with_symb,SPdeduction) (DYmultranrel,DYdeduction) composeDedOverApproxSapic),wded3Sp) wded4Sp
+        (Sym,((IMAGE INL (IMAGE (SUM_MAP translate_BinPred_to_SPpred I) P)):((SPpred + DYpred) + (SPpred + DYpred) -> bool)),((Pconfig ((symbtree_to_sapic iT0),0,iRe0,iNRe0)),ESt),((Pconfig ((symbtree_to_sapic rT0),0,rRe0,rNRe0)),ESt))
+        (Sym',((IMAGE INL (IMAGE (SUM_MAP translate_BinPred_to_SPpred I) P')):((SPpred + DYpred) + (SPpred + DYpred) -> bool)),((Pconfig ((symbtree_to_sapic iTre),ii,iRe,iNRe)),ESt),((Pconfig ((symbtree_to_sapic rTre),ri,rRe,rNRe)),ESt)))
        =
        (IMAGE (MAP (OPTION_MAP INL))
-        (comptraces_sapic (sapic_position_multi_transitions_with_symb,sapic_Ded) (DYmultranrel,DYdeduction) composeDedOverApproxSapic (Sym,(IMAGE (SUM_MAP translate_birexp_to_sapicterm I) P),(Pconfig ((ProcessComb Parallel (symbtree_to_sapic iT0) (symbtree_to_sapic rT0)),0,(sapic_renaming_extend iRe0 rRe0),(sapic_name_renaming_extend iNRe0 rNRe0))),ESt) (Sym',(IMAGE (SUM_MAP translate_birexp_to_sapicterm I) P'),(Pconfig ((ProcessComb Parallel (symbtree_to_sapic iTre) (symbtree_to_sapic rTre)),(ii + ri),(sapic_renaming_extend iRe rRe),( sapic_name_renaming_extend iNRe rNRe))),ESt)))
+        (comptraces_sapic (sapic_position_multi_transitions_with_symb,SPdeduction) (DYmultranrel,DYdeduction) composeDedOverApproxSapic (Sym,(IMAGE (SUM_MAP translate_BinPred_to_SPpred I) P),(Pconfig ((ProcessComb Parallel (symbtree_to_sapic iT0) (symbtree_to_sapic rT0)),0,(sapic_renaming_extend iRe0 rRe0),(sapic_name_renaming_extend iNRe0 rNRe0))),ESt) (Sym',(IMAGE (SUM_MAP translate_BinPred_to_SPpred I) P'),(Pconfig ((ProcessComb Parallel (symbtree_to_sapic iTre) (symbtree_to_sapic rTre)),(ii + ri),(sapic_renaming_extend iRe rRe),( sapic_name_renaming_extend iNRe rNRe))),ESt)))
        ) ==>
-       (comptraces (sapic_position_multi_transitions_with_symb,sapic_Ded) (DYmultranrel,DYdeduction) composeDedOverApproxSapic (Sym,(IMAGE (SUM_MAP translate_birexp_to_sapicterm I) P),(Pconfig ((ProcessComb Parallel (symbtree_to_sapic iT0) (symbtree_to_sapic rT0)),0,(sapic_renaming_extend iRe0 rRe0),(sapic_name_renaming_extend iNRe0 rNRe0))),ESt) (Sym',(IMAGE (SUM_MAP translate_birexp_to_sapicterm I) P'),(Pconfig ((ProcessComb Parallel (symbtree_to_sapic iTre) (symbtree_to_sapic rTre)),(ii + ri),(sapic_renaming_extend iRe rRe),(sapic_name_renaming_extend iNRe rNRe))),ESt)) 
+       (comptraces (sapic_position_multi_transitions_with_symb,SPdeduction) (DYmultranrel,DYdeduction) composeDedOverApproxSapic (Sym,(IMAGE (SUM_MAP translate_BinPred_to_SPpred I) P),(Pconfig ((ProcessComb Parallel (symbtree_to_sapic iT0) (symbtree_to_sapic rT0)),0,(sapic_renaming_extend iRe0 rRe0),(sapic_name_renaming_extend iNRe0 rNRe0))),ESt) (Sym',(IMAGE (SUM_MAP translate_BinPred_to_SPpred I) P'),(Pconfig ((ProcessComb Parallel (symbtree_to_sapic iTre) (symbtree_to_sapic rTre)),(ii + ri),(sapic_renaming_extend iRe rRe),(sapic_name_renaming_extend iNRe rNRe))),ESt)) 
        =
-       (sapic_plus_traces sapic_plus_position_multi_transitions_with_symb (Sym,(IMAGE (SUM_MAP translate_birexp_to_sapicterm I) P),(Pconfig_plus ((ProcessComb Parallel (symbtree_to_sapic iT0) (symbtree_to_sapic rT0)),0,(sapic_renaming_extend iRe0 rRe0),(sapic_name_renaming_extend iNRe0 rNRe0)))) (Sym',(IMAGE (SUM_MAP translate_birexp_to_sapicterm I) P'),(Pconfig_plus ((ProcessComb Parallel (symbtree_to_sapic iTre) (symbtree_to_sapic rTre)),(ii + ri),(sapic_renaming_extend iRe rRe),( sapic_name_renaming_extend iNRe rNRe)))))
+       (sapic_plus_traces sapic_plus_position_multi_transitions_with_symb (Sym,(IMAGE (SUM_MAP translate_BinPred_to_SPpred I) P),(Pconfig_plus ((ProcessComb Parallel (symbtree_to_sapic iT0) (symbtree_to_sapic rT0)),0,(sapic_renaming_extend iRe0 rRe0),(sapic_name_renaming_extend iNRe0 rNRe0)))) (Sym',(IMAGE (SUM_MAP translate_BinPred_to_SPpred I) P'),(Pconfig_plus ((ProcessComb Parallel (symbtree_to_sapic iTre) (symbtree_to_sapic rTre)),(ii + ri),(sapic_renaming_extend iRe rRe),( sapic_name_renaming_extend iNRe rNRe)))))
     )
 
     ``,
