src/tools/parallelcomposition/instantiations/sbir_sapic_comp_DYScript.sml
@@ -21,11 +21,11 @@ val _ = new_theory "sbir_sapic_comp_DY";
 val comptraces_sapic_def =
 Define`
       comptraces_sapic
-      ((MTrn1:(SapicFact_t + (Name_t,Sig_t,Var_t) sync_event, SapicTerm_t, sapic_position_configuration_t, Var_t) mtrel),(Ded1:(SapicTerm_t) tded))
+      ((MTrn1:(SapicFact_t + (Name_t,Sig_t,Var_t) sync_event, SPpred, sapic_position_configuration_t, Var_t) mtrel),(Ded1:(SPpred) tded))
       ((MTrn2:(DYnsyc_event + (Name_t,Sig_t,Var_t) sync_event, DYpred, DYstate, Var_t) mtrel),(Ded2:(DYpred) tded))
       ded3
-      ((Sym:Var_t set),(P: (SapicTerm_t + DYpred) set),(S1: sapic_position_configuration_t),(S2: DYstate))
-      ((Sym':Var_t set),(P': (SapicTerm_t + DYpred) set),(S1': sapic_position_configuration_t),(S2': DYstate))
+      ((Sym:Var_t set),(P: (SPpred + DYpred) set),(S1: sapic_position_configuration_t),(S2: DYstate))
+      ((Sym':Var_t set),(P': (SPpred + DYpred) set),(S1': sapic_position_configuration_t),(S2': DYstate))
 =
 {(t:((SapicFact_t + (Name_t,Sig_t,Var_t) sync_event)+(DYnsyc_event + (Name_t,Sig_t,Var_t) sync_event)) option list)|  
  (symbolicParlComp (MTrn1,Ded1) (MTrn2,Ded2) ded3 (Sym,P,S1,S2) t (Sym',P',S1',S2'))
@@ -121,14 +121,14 @@ val binterl_sbir_to_sapic_thm = store_thm(
 
 val compose_sbir_sapic_vs_DY_thm = store_thm(
   "compose_sbir_sapic_vs_DY_thm",
-  ``∀T0 Re0 NRe0 i Re NRe Tre (Sym:(Var_t -> bool)) (Sym':(Var_t -> bool)) (P:(bir_exp_t + DYpred -> bool)) (P':(bir_exp_t + DYpred -> bool)) (DedTr:(bir_exp_t) tded) (DedSp:(SapicTerm_t) tded).
+  ``∀T0 Re0 NRe0 i Re NRe Tre (Sym:(Var_t -> bool)) (Sym':(Var_t -> bool)) (P:(bir_exp_t + DYpred -> bool)) (P':(bir_exp_t + DYpred -> bool)) (DedTr:(bir_exp_t) tded).
 (
-((IMAGE (MAP sbirEvent_vs_Sync_to_sapicFact_vs_Sync) (traces_of_tree_with_symb (Sym,IMAGE OUTL P,T0) (Sym',IMAGE OUTL P',Tre))) ⊆ (traces_of_sapic_with_symb (Sym,IMAGE OUTL (IMAGE (SUM_MAP translate_birexp_to_sapicterm I) P),(Pconfig ((symbtree_to_sapic T0),0,Re0,NRe0))) (Sym',IMAGE OUTL (IMAGE (SUM_MAP translate_birexp_to_sapicterm I) P'),(Pconfig ((symbtree_to_sapic Tre),i,Re,NRe))))) ∧
+((IMAGE (MAP sbirEvent_vs_Sync_to_sapicFact_vs_Sync) (traces_of_tree_with_symb (Sym,IMAGE OUTL P,T0) (Sym',IMAGE OUTL P',Tre))) ⊆ (traces_of_sapic_with_symb (Sym,IMAGE OUTL (IMAGE (SUM_MAP translate_BinPred_to_SPpred I) P),(Pconfig ((symbtree_to_sapic T0),0,Re0,NRe0))) (Sym',IMAGE OUTL (IMAGE (SUM_MAP translate_BinPred_to_SPpred I) P'),(Pconfig ((symbtree_to_sapic Tre),i,Re,NRe))))) ∧
         (TransDisable composeDedOverApprox (symbolic_tree_multi_transitions_with_symb,DedTr) (DYmultranrel,DYdeduction)) ∧
-      (TransEnable composeDedOverApproxSapic (sapic_position_multi_transitions_with_symb,DedSp) (DYmultranrel,DYdeduction))
+      (TransEnable composeDedOverApproxSapic (sapic_position_multi_transitions_with_symb,SPdeduction) (DYmultranrel,DYdeduction))
     ) ==> (
       (IMAGE (MAP sbirEvent_vs_DY_to_sapicFact_vs_DY) (comptraces_tree (symbolic_tree_multi_transitions_with_symb,DedTr) (DYmultranrel,DYdeduction) composeDedOverApprox (Sym,P,T0,ESt) (Sym',P',Tre,ESt))) ⊆
-      (comptraces_sapic (sapic_position_multi_transitions_with_symb,DedSp) (DYmultranrel,DYdeduction) composeDedOverApproxSapic (Sym,(IMAGE (SUM_MAP translate_birexp_to_sapicterm I) P),(Pconfig ((symbtree_to_sapic T0),0,Re0,NRe0)),ESt) (Sym',(IMAGE (SUM_MAP translate_birexp_to_sapicterm I) P'),(Pconfig ((symbtree_to_sapic Tre),i,Re,NRe)),ESt))
+      (comptraces_sapic (sapic_position_multi_transitions_with_symb,SPdeduction) (DYmultranrel,DYdeduction) composeDedOverApproxSapic (Sym,(IMAGE (SUM_MAP translate_BinPred_to_SPpred I) P),(Pconfig ((symbtree_to_sapic T0),0,Re0,NRe0)),ESt) (Sym',(IMAGE (SUM_MAP translate_BinPred_to_SPpred I) P'),(Pconfig ((symbtree_to_sapic Tre),i,Re,NRe)),ESt))
       ) ``,
         rpt gen_tac >>      
      rewrite_tac[binterleave_ts,traces_def,comptraces_def,EXTENSION,traces_of_tree_with_symb_def,traces_of_sapic_with_symb_def,EXTENSION,SUBSET_DEF,comptraces_tree_def, comptraces_sapic_def,binterleave_ts] >>
